veric/expr_lemmas.v
@@ -18,8 +18,9 @@ Definition empty_tenv := PTree.empty val.
 Definition empty_environ : environ :=
 mkEnviron (filter_genv empty_genv) (Map.empty _) (Map.empty _).
 
-Definition Delta1 : tycontext := (PTree.set 1%positive (type_int32s, false) (PTree.empty (type * bool)),
-                                 PTree.empty type, Tvoid,nil).
+Definition Delta1 : tycontext := (PTree.set 1%positive (type_int32s, false) 
+                                 (PTree.empty (type * bool)),
+                                 PTree.empty type, Tvoid,PTree.empty _).
 
 Lemma Zlt_bool_rev: forall x y, Zlt_bool x y = Zgt_bool y x.
 Proof.
@@ -83,22 +84,28 @@ Qed.
 Definition tc_te_denote (te: tenviron) (tc: PTree.t (type * bool)) :=
 forall id ty b, tc ! id = Some (ty,b) -> exists v, (Map.get te id = Some v /\ typecheck_val v ty = true). 
 
-Definition tc_vl_denote (ve:venviron) le := forall id,
-(In id le -> Map.get ve id = None).
+Definition tc_ve_denote (ve: venviron) (tc: PTree.t type) :=
+forall id ty, tc ! id = Some (ty) ->
+exists v, Map.get ve id = Some(v,ty).
 
-(*This one is a little intense, but it has to deal with the way vars "override"
-globals. Even if globals aren't visible behind vars they still need to be typed
-correctly *)
-Definition tc_ve_denote (ve: venviron) (ge:genviron) (tc: PTree.t type) :=
-forall id ty, tc ! id = Some (ty) -> 
-((exists v, (Map.get ve  id = Some(v, ty))) \/
+Definition tc_mode_denote (rho:environ) (Delta:tycontext)  :=
+forall id t, (glob_types Delta) ! id = Some t ->
+(ve_of rho) id = None \/ exists t,  (var_types Delta) ! id = Some t. 
+
+
+Definition tc_ge_denote (ge: genviron) (tc: PTree.t global_spec) :=
+forall id  t,  tc ! id = Some t -> 
+((exists b, exists i, 
+(ge id = Some (Vptr b i, globtype t) /\ typecheck_val (Vptr b i) (globtype t) = true))).
+
+(*((exists v, (Map.get ve  id = Some(v, ty))) \/
 ((exists b, exists i, 
 (ge id = Some (Vptr b i, ty) /\ typecheck_val (Vptr b i) ty = true)
  /\ (exists v, (Map.get ve id = Some(v, ty)))) \/
 ((exists b, exists i, 
 (ge id = Some (Vptr b i, ty) /\ typecheck_val (Vptr b i) ty = true)
  /\ (Map.get ve  id = None)))))
-.
+.*)
 
 Lemma eqb_type_eq: forall t1 t2, eqb_type t1 t2 = proj_sumbool (type_eq t1 t2).
 Proof.
@@ -112,25 +119,8 @@ auto.
 Qed.
 
 
-(*Delete if this file builds
-Lemma fold_left_false : forall T l f, 
-fold_left (fun (a:bool) (p: T) => f p && a) l false = false.
-Proof.
-intros.
-induction l. auto. simpl in *. rewrite andb_false_r. auto.
-Qed.
 
-Lemma fold_left_forallb : forall T l f, 
-fold_left (fun (a:bool) (p:T) => f p && a) l true = forallb f l.
-Proof.
-intros.
-induction l; auto. simpl. destruct (f a). simpl. auto. simpl. apply fold_left_false.
-Qed.
-*)
-
-(*environment typecheck soundness*)
-
-Lemma typecheck_vl_eqv : forall vl ve, 
+(*Lemma typecheck_vl_eqv : forall vl ve, 
 typecheck_non_var_list vl ve = true <->
 tc_vl_denote ve vl.
 Proof.
@@ -149,84 +139,138 @@ apply IHvl; auto. intros. simpl in H. specialize (H x). intuition.
 unfold tc_vl_denote in *. unfold typecheck_non_var_list. rewrite forallb_forall.
 intros. specialize (H x). intuition. rewrite H1. auto.
 Qed.
+*)
+
+Lemma In_fst_split : forall A B i (l: list (A * B)), In i (fst (split l)) <-> exists b : B, In (i,b) l.  
+Proof. 
+intros. split; intros. induction l. inv H. simpl in H. remember (split l). destruct p. destruct a. 
+simpl in *. destruct H. subst. clear IHl. eauto.
+destruct IHl. auto. exists x. auto. 
+
+induction l. destruct H. inv H. simpl in *. destruct H. destruct H. destruct a. inv H.
+clear IHl. destruct (split l). simpl. auto. destruct (split l). destruct a. simpl. 
+right. apply IHl. eauto. 
+Qed.
 
 
-Lemma typecheck_ve_eqv : forall dv ve ge,
-typecheck_var_environ (PTree.elements dv) ve ge = true <->
-tc_ve_denote ve ge dv.
+Lemma typecheck_mode_eqv : forall rho Delta,
+same_env rho Delta (all_var_ids Delta) = true <->
+tc_mode_denote rho Delta. 
+Proof.
+intros. split; intros. unfold all_var_ids in H.
+intro. intros.
+assert (In id  (fst (split (PTree.elements (glob_types Delta))))). 
+rewrite In_fst_split. exists t. apply PTree.elements_correct. auto. 
+
+induction (fst (split (PTree.elements (glob_types Delta)))). unfold same_env in *. 
+congruence.
+
+simpl in H. rewrite andb_true_iff in *. destruct H. 
+simpl in H1. destruct H1. subst. unfold same_mode in H. 
+remember ((var_types Delta) ! id). destruct o. eauto.
+remember ((glob_types Delta) ! id). destruct o. 
+remember (ve_of rho id). destruct o; try congruence. auto. congruence.
+destruct IHl; auto. 
+
+unfold tc_mode_denote in *. unfold all_var_ids in *. 
+assert (forall id, In id  (fst (split (PTree.elements (glob_types Delta)))) ->
+    exists t, ((glob_types Delta) ! id) = Some t).
+intros. rewrite In_fst_split in H0. destruct H0. 
+apply PTree.elements_complete in H0. eauto.
+
+induction  (fst (split (PTree.elements (glob_types Delta)))).
+simpl in *.  (*SDLFKJSDFLKJ:DSKLGJS:LDKJ:GDLkj check use before I hack at this mroe*)
+Admitted.
+
+Lemma typecheck_ve_eqv : forall dv ve,
+typecheck_var_environ (PTree.elements dv) ve  = true <->
+tc_ve_denote ve dv.
 Proof.
 intros; split; intros.
-unfold tc_ve_denote. intros. 
-assert (In (id, ty) (PTree.elements dv)). apply PTree.elements_correct.
-auto.
-assert (forall t: type, In (id,t) (PTree.elements dv) -> dv ! id = Some t).
-intros. apply PTree.elements_complete. auto. 
-
-
-
+unfold tc_ve_denote. intros.   
 assert (In (id, ty) (PTree.elements dv)). apply PTree.elements_correct.
 auto.
 assert (forall t: type, In (id,t) (PTree.elements dv) -> dv ! id = Some t).
 intros. apply PTree.elements_complete. auto.
-induction (PTree.elements dv). inv H1. 
-simpl in H. destruct a. simpl in *.
-remember (Map.get ve p). destruct o. destruct p0.
-remember (eqb_type t t0). destruct b0.
-symmetry in Heqb0. apply eqb_type_true in Heqb0. subst.
-destruct H1. inv H1. specialize (H2 ty). intuition; eauto.
+ induction (PTree.elements dv). 
+  inv H1. 
+  simpl in H. destruct a. simpl in *.
+    remember (Map.get ve p). destruct o. 
+       destruct p0.
+             remember (eqb_type t t0). destruct b0.
+             symmetry in Heqb0. apply eqb_type_true in Heqb0. subst.
+             destruct H1. inv H1. specialize (H2 ty). intuition; eauto.
 
-apply IHl; eauto.
+             apply IHl; eauto.
 
-simpl in *; congruence.
+             simpl in *; congruence.
 
-remember (ge p). destruct o; simpl in *; try congruence. destruct p0.
-destruct v; simpl in *; try congruence. remember (eqb_type t t0).
-destruct b0; simpl in *; try congruence. symmetry in Heqb0.
- apply eqb_type_true in Heqb0; subst.
-simpl in *. destruct H1. inv H1. right. right. exists b. exists i.
-intuition. destruct ty; auto. if_tac in H; try congruence.
-intuition. destruct H5; auto. destruct H3. rewrite <- Heqo in H3. congruence. 
-destruct H3. destruct H3. destruct H3. intuition.
-destruct H3. destruct H3; intuition.
-apply IHl; auto. destruct t0; auto; simpl in *; congruence.
+       simpl in *. congruence.
 
+
+ 
 (*other way now...*)
 assert (forall t1 id, In (id,t1) (PTree.elements dv) -> dv ! id = Some t1).
 intros. apply PTree.elements_complete. auto.
 induction (PTree.elements dv).
-auto.
+  auto.
 
-simpl in *. destruct a. 
-remember (Map.get ve p). destruct o. destruct p0.
-simpl in *. unfold tc_ve_denote in H.
+  simpl in *. destruct a. 
+    remember (Map.get ve p). destruct o. 
+      destruct p0.
+        simpl in *. unfold tc_ve_denote in H.
 
-assert (forall (t1 : type) (id : positive),
-     (p, t) = (id, t1) \/ In (id, t1) l -> dv ! id = Some t1) by auto.
-specialize (H0 t p). intuition. specialize (H _ _ H0).
-destruct H. destruct H. rewrite H in Heqo. inv Heqo.
-rewrite eqb_type_refl. simpl. apply IHl. intros. apply H1. auto.
+        assert (forall (t1 : type) (id : positive),
+          (p, t) = (id, t1) \/ In (id, t1) l -> dv ! id = Some t1) by auto.
+        specialize (H0 t p). intuition. specialize (H _ _ H0).
+        destruct H.  rewrite H in Heqo.  inv Heqo.
+        rewrite eqb_type_refl. simpl. apply IHl. intros. apply H1. auto.
 
-destruct H. destruct H. destruct H. destruct H. destruct H.
-destruct H2. rewrite H2 in Heqo. inv Heqo. rewrite eqb_type_refl.
-simpl. apply IHl. intros. apply H1. auto.
+      simpl. spec IHl. intros. apply H0. auto. unfold tc_ve_denote in H.
+          edestruct H. auto. congruence. Qed.
+ 
+Lemma typecheck_ge_eqv : forall dv ge,
+typecheck_glob_environ (PTree.elements dv) ge = true <-> tc_ge_denote ge dv.
+Proof.
+intros.  
 
-repeat destruct H. rewrite H2 in Heqo. congruence.
+split; intros. 
+  unfold tc_ge_denote. intros. 
+   assert (In (id,t)  (PTree.elements dv)). 
+        apply PTree.elements_correct. auto. 
+   assert (forall t: global_spec, In (id,t) (PTree.elements dv) -> dv ! id = Some t).
+    intros. apply PTree.elements_complete. auto. 
+   
+   induction (PTree.elements dv). 
+    inv H1. 
+    simpl in H1. destruct a. simpl in H. remember (ge p). destruct o; try congruence.
+    destruct p0. destruct v; try congruence. remember (eqb_type (globtype g) t0).
+    destruct b0; simpl in H; try congruence. 
+    symmetry in Heqb0. apply eqb_type_true in Heqb0. subst. 
+    assert (typecheck_glob_environ l ge = true).
+      simpl in H.  if_tac in H; try congruence. 
+    destruct H1.  
+      inv H1. rewrite <- Heqo. eexists;  eexists. split. auto. 
+      remember (globtype t). destruct t0; simpl in H; try congruence; auto. 
+    destruct IHl; auto. intros. apply H2. simpl; auto.
+    destruct H4. destruct H4. eauto. 
 
-remember (ge p). destruct o. destruct p0. rewrite IHl; auto.
-specialize (H0 t p). intuition.
-unfold tc_ve_denote in *. edestruct H; eauto.
-destruct H1. rewrite <- Heqo in H1. congruence. destruct H1.
-repeat destruct H1. destruct H3. rewrite <- Heqo in H1. congruence.
+   unfold tc_ge_denote in *. 
+   assert (forall t1 id, In (id,t1) (PTree.elements dv) -> dv ! id = Some t1).
+    intros. apply PTree.elements_complete. auto.
+   induction (PTree.elements dv). 
+     auto. 
+     
+     simpl. destruct a. rewrite IHl; auto. 
+     clear IHl. unfold Map.get in H. edestruct H.  apply H0. simpl. left.
+     auto. destruct H1 as [i [? ?]]. rewrite H1. rewrite eqb_type_refl.
+     simpl. destruct (globtype g); simpl in H2; try congruence; auto. 
 
-destruct H1. destruct H1. destruct H1. destruct H1.
-rewrite <- Heqo0 in H1. inv H1. rewrite eqb_type_refl. simpl. destruct t; auto; congruence.
-specialize (H0 t p). intuition. clear H2. unfold tc_ve_denote in *.
-specialize (H _ _ H0). destruct H. destruct H. rewrite H in *; congruence.
-destruct H. repeat destruct H. destruct H1. rewrite H in *; congruence.
-destruct H. destruct H. destruct H. destruct H. rewrite H in *; congruence.
-
+     intros; auto. 
+     apply H0; auto. simpl; auto. 
 Qed. 
-
+     
+   
 Lemma typecheck_te_eqv : forall t te, typecheck_temp_environ (PTree.elements t) te = true
 <-> tc_te_denote te t.
 Proof. intros.
@@ -261,8 +305,8 @@ Qed.
 
 Lemma typecheck_environ_sound : forall ge te ve Delta,
 typecheck_environ (mkEnviron ge ve te) Delta = true ->
-tc_te_denote te (temp_types Delta) /\ tc_ve_denote ve ge (var_types Delta) /\ 
-tc_vl_denote ve (non_var_ids Delta).
+tc_te_denote te (temp_types Delta) /\ tc_ve_denote ve (var_types Delta) /\ 
+tc_ge_denote ge (glob_types Delta).
 Proof.
 intros.
 unfold typecheck_environ in *. destruct Delta. destruct p.
@@ -272,13 +316,13 @@ destruct p. simpl in *. apply typecheck_te_eqv; auto.
 
 apply typecheck_ve_eqv; auto.
 
-apply typecheck_vl_eqv; auto.
+apply typecheck_ge_eqv; auto.
 
 Qed.
 
 
 (*Lemmas about soundness of environment join*)
-
+(*
 Lemma join_ve_denote : forall ve1 ve2 id v1,
 (join_ve ve1 ve2) ! id = Some (v1) ->
 ve1 ! id = Some (v1) /\ ve2 ! id = Some (v1).
@@ -304,7 +348,7 @@ apply IHl; eauto.
 apply IHl; eauto.
 apply IHl; eauto. intros. apply H0. simpl. eauto.
 Qed.
-
+*)
 
 Lemma join_te_denote : forall te1 te2 id b t1,
 (join_te te1 te2) ! id = Some (t1,b) ->
@@ -343,6 +387,7 @@ apply IHl; eauto.
 apply IHl; eauto.
 Qed.
 
+(*
 Lemma join_vl_denote :  forall vl1 vl2 id,
 In id (join_ve_list vl1 vl2) -> In id vl1 /\ In id vl2.
 Proof.
@@ -351,65 +396,81 @@ induction vl1. simpl in *. inv H. simpl in *. if_tac in H. simpl in *; intuition
 subst; auto. intuition.
 
 Qed.
+*)
+
+(*Lemma join_ve_same : forall ve,
+join_ve ve ve = ve. *)
+
+
+Lemma same_env_ignores_t_ret : forall e0 e1 e2 e3 e4 e5 rho,
+same_env rho (e1,e2,e3,e4) (all_var_ids (e1,e2,e3,e4)) =
+ same_env rho (e0,e2,e5,e4) (all_var_ids (e0,e2,e5,e4)).  
+intros. unfold all_var_ids. simpl. induction (fst (split (PTree.elements e4))). 
+auto. simpl. rewrite IHl.  auto. Qed.
+
+
+Lemma same_env_ignores_te : forall te te1 ve ge Delta,
+same_env (mkEnviron ge ve te) Delta (all_var_ids Delta) =
+same_env (mkEnviron ge ve te1) Delta (all_var_ids Delta). 
+intros. induction (all_var_ids Delta). auto.
+simpl. rewrite IHl. auto.
+Qed.
 
 Lemma typecheck_environ_join1:
   forall rho Delta1 Delta2, 
+        var_types Delta1 = var_types Delta2 ->
+        glob_types Delta1 = glob_types Delta2 ->
+    
         typecheck_environ rho Delta1 = true ->
         typecheck_environ rho (join_tycon Delta1 Delta2) = true.
 Proof. intros.
- unfold typecheck_environ in *. rewrite andb_true_iff in *. intuition.
-destruct rho. simpl in *. rewrite andb_true_iff in *; intuition.
-rewrite  typecheck_te_eqv in *. clear H1. clear H2.
+ unfold typecheck_environ in *. repeat rewrite andb_true_iff in *. intuition.
+destruct rho. simpl in *. 
+rewrite  typecheck_te_eqv in *. clear H3 H4 H5. 
 unfold tc_te_denote in *. intros. unfold temp_types in *.
 destruct Delta2. destruct p. destruct p. simpl in *. destruct Delta0.
-destruct p. destruct p. simpl in *. apply join_te_denote in H0.
-destruct H0. destruct H0. destruct H1. 
-eapply H. apply H0.
+destruct p. destruct p. simpl in *. apply join_te_denote in H1.
+destruct H1. destruct H1. destruct H3. 
+eapply H2. eauto.  
+unfold join_tycon. destruct Delta2. 
+destruct p. destruct p. destruct Delta0. destruct p. destruct p.
+unfold join_te. unfold var_types in *.  simpl in *. subst. auto. 
 
-clear H. clear H1. rewrite typecheck_ve_eqv in *.
-destruct Delta1. simpl. destruct p. destruct Delta2. destruct p.
-unfold var_types in *. simpl in *. destruct p0.
-destruct p. destruct Delta0. destruct p. destruct p.
-simpl in *.
-unfold tc_ve_denote in *.
-intros. apply join_ve_denote in H. destruct H.
-intuition.
+unfold join_tycon. destruct Delta2. destruct p. destruct p. destruct Delta0.
+repeat destruct p. unfold glob_types in *; simpl in *; subst; auto. 
 
-clear H0. rewrite typecheck_vl_eqv in *.
-destruct Delta2; destruct Delta0. destruct p.
-destruct p. destruct p0. destruct p. unfold ve_of in *; simpl in *.
-destruct rho. unfold tc_vl_denote in *. intros.
-apply H1.  
-apply join_vl_denote in H. intuition.
-Qed.
+unfold join_tycon. destruct Delta2. destruct p. destruct p. destruct Delta0.
+repeat destruct p. erewrite same_env_ignores_t_ret. eauto. 
+Qed. 
+
 
 Lemma typecheck_environ_join2:
   forall rho Delta1 Delta2, 
+        var_types Delta1 = var_types Delta2 ->
+        glob_types Delta1 = glob_types Delta2 ->
         typecheck_environ rho Delta2 = true ->
         typecheck_environ rho (join_tycon Delta1 Delta2) = true.
 Proof.
-intros. unfold typecheck_environ in *. repeat rewrite andb_true_iff in *.
-intuition.
-clear H1. clear H2. rewrite typecheck_te_eqv in *.
-unfold tc_te_denote in *; intros. unfold temp_types in *. destruct Delta2.
-destruct p. destruct Delta0. destruct p. destruct p0. destruct p. simpl in *.
-apply join_te_denote in H0. destruct H0. destruct H0. destruct H1.
-destruct rho; simpl in *. eapply H. eauto.
+intros.
+ unfold typecheck_environ in *. repeat rewrite andb_true_iff in *. intuition.
+destruct rho. simpl in *. 
+rewrite  typecheck_te_eqv in *. clear H4 H5. 
+unfold tc_te_denote in *. intros. unfold temp_types in *.
+destruct Delta2. destruct p. destruct p. simpl in *. destruct Delta0.
+destruct p. destruct p. simpl in *. apply join_te_denote in H1.
+destruct H1. destruct H1. destruct H4. 
+eauto. 
+unfold join_tycon. destruct Delta2. 
+destruct p. destruct p. destruct Delta0. destruct p. destruct p.
+unfold join_te. unfold var_types in *.  simpl in *. subst. auto. 
 
-clear H. rewrite typecheck_ve_eqv in *.
-destruct Delta1. simpl. destruct p. destruct Delta2. destruct p.
-unfold var_types in *.
-destruct p0. destruct p. destruct Delta0. destruct p. destruct p.
- simpl in *. unfold tc_ve_denote in *.
-intros. apply join_ve_denote in H. destruct H.
-intuition.
+unfold join_tycon. destruct Delta2. destruct p. destruct p. destruct Delta0.
+repeat destruct p. unfold glob_types in *; simpl in *; subst; auto. 
 
-clear H. clear H2. rewrite typecheck_vl_eqv in *.
-destruct Delta2; destruct Delta0. destruct p.
-destruct p. destruct p0. destruct p. unfold ve_of in *; simpl in *.
-destruct rho. unfold tc_vl_denote in *. intros.
-apply H1.  
-apply join_vl_denote in H. intuition.
+unfold join_tycon. destruct Delta2. destruct p. destruct p. destruct Delta0.
+repeat destruct p. unfold var_types in *. simpl in H. subst. unfold glob_types in *.
+simpl in *. subst.  erewrite same_env_ignores_t_ret. eauto.
+
 Qed.
 
 Lemma typecheck_val_ptr_lemma:
@@ -420,9 +481,9 @@ Lemma typecheck_val_ptr_lemma:
    typecheck_val (eval_id id rho) (Tpointer t a) = true.
 Proof. 
 intros. unfold bool_val in *. unfold typecheck_val.
-unfold eval_id. apply typecheck_environ_sound in H.
+unfold eval_id. destruct rho.  apply typecheck_environ_sound in H.
 destruct H as [? _]. unfold tc_te_denote in *.
-edestruct H; eauto. destruct H2. rewrite H2. destruct x; simpl in *; congruence.
+edestruct H; eauto. destruct H2.  simpl.  rewrite H2. destruct x; simpl in *; congruence.
 Qed. 
 
 
@@ -433,12 +494,17 @@ typecheck_environ (mkEnviron ge ve te) Delta = true ->
 typecheck_environ (mkEnviron ge ve (Map.set id v te)) Delta = true.
 Proof. 
 intros. unfold typecheck_environ in *. simpl in *. repeat rewrite andb_true_iff in *.
-intuition. clear H2 H3. destruct Delta. destruct p. destruct p. unfold temp_types in *; simpl in *.
-clear t t1 l ve. rewrite typecheck_te_eqv in *. unfold tc_te_denote in *.
-intros. edestruct H; eauto. destruct H2. rewrite Map.gsspec.
+intuition. clear H2 H3. destruct Delta. destruct p. 
+destruct p. unfold temp_types in *; simpl in *.
+rewrite typecheck_te_eqv in *. unfold tc_te_denote in *.
+intros. edestruct H1; eauto. destruct H2. rewrite Map.gsspec.
 if_tac. subst. exists v; intuition. specialize (H0 (ty, b)). apply H0. auto. 
 
 simpl in *. exists x. intuition.
+
+erewrite same_env_ignores_te. eauto. 
+
+
 Qed.
 
 
@@ -455,38 +521,26 @@ apply typecheck_environ_put_te; auto.
 unfold typecheck_environ in *. simpl in *. repeat rewrite andb_true_iff in *. intuition.
 
 destruct Delta. destruct p. destruct p.  unfold initialized. unfold temp_types in *.
-clear H4 H3 H5 H6. simpl in *. 
-rewrite typecheck_te_eqv in *. unfold tc_te_denote in *. intros. remember (t0 ! id).
-destruct o; try congruence; auto. destruct p. simpl in *. rewrite PTree.gsspec in H.
-if_tac in H. inv H. eapply H2; eauto.
+clear H4 H3 H5 H6 H7 H8. simpl in *. 
+rewrite typecheck_te_eqv in *. unfold tc_te_denote in *. intros. remember (t1 ! id).
+destruct o; try congruence; auto. destruct p. simpl in *. rewrite PTree.gsspec in H2.
+if_tac in H2. inv H2. eauto. eauto. eauto.
 
-rewrite Map.gsspec. if_tac; intuition. eauto.
-
-simpl in *. eapply H2; eauto.
 
 unfold var_types in *. destruct Delta. destruct p. destruct p. simpl in *.
-unfold initialized. simpl. destruct ((temp_types (t0, t1, t, l))!id).
+unfold initialized. simpl. destruct ((temp_types (t1, t2, t0, t))!id).
 destruct p. simpl. unfold var_types. auto. auto.
 
 destruct Delta. destruct p. destruct p. simpl in *. unfold initialized.
-destruct ((temp_types (t0, t1, t, l)) ! id); try destruct p;
-unfold non_var_ids; simpl in *; auto.
+destruct ((temp_types (t1, t2, t0, t)) ! id); try destruct p; simpl in *; auto.
+
+erewrite same_env_ignores_te; eauto. unfold initialized.
+destruct Delta. simpl in *.  destruct p. destruct p. 
+unfold var_types, temp_types in *. simpl in *. 
+destruct (t1 ! id); try destruct p;
+try erewrite same_env_ignores_t_ret;  eauto.
+
 Qed. 
-
-(*
-Lemma no_rep_in_pair : forall A B L a b b2, list_norepet (map (@fst A B) (L)) ->
-  In (a, b) L -> In (a,b2) L -> b = b2.
-Proof.
-intros A B L. induction L; intros. inv H0. simpl in *.
-inv H. intuition.
-  destruct a. inv H0. inv H. auto.
- 
-  destruct H4. destruct a; simpl. inv H. eapply in_fst_in. eauto. 
-  
-  destruct H4. destruct a; simpl. inv H0. eapply in_fst_in. eauto.
-
-  eapply IHL; eauto.
-Qed. *)
 
 Lemma type_eq_true : forall a b, proj_sumbool  (type_eq a b) =true  -> a = b.
 Proof. intros. destruct (type_eq a b). auto. simpl in H. inv H.
@@ -547,7 +601,8 @@ Qed.
 
 Lemma eval_lvalue_ptr : forall rho e (Delta: tycontext) te ve ge,
 mkEnviron ge ve te = rho -> 
-tc_ve_denote ve ge (var_types Delta) -> 
+tc_ve_denote ve (var_types Delta) -> 
+tc_ge_denote ge (glob_types Delta) ->
 denote_tc_assert (typecheck_lvalue Delta e) rho ->
 eval_lvalue e rho = Vundef \/ exists base, exists ofs, eval_lvalue e rho  = Vptr base ofs.
 Proof. 
@@ -562,22 +617,26 @@ remember (ge_of rho i); try rewrite eqb_type_eq; simpl.
 destruct o; try rewrite eqb_type_eq; simpl; eauto.
 destruct p; try rewrite eqb_type_eq; simpl; eauto.
 if_tac; eauto.
-unfold tc_ve_denote in *. simpl in H1.
+unfold tc_ve_denote in *. simpl in H2.
+unfold get_var_type in *. 
 remember ((var_types Delta) ! i).
-destruct o. subst. simpl in H1.
-unfold lift2 in H1.
-try rewrite eqb_type_eq in H1; simpl in *; intuition.
+destruct o. subst. simpl in H2.
+unfold lift2 in *.
+try rewrite eqb_type_eq in *; simpl in *; intuition.
 symmetry in Heqo1.
 specialize (H0 i t1 Heqo1).
-destruct H0. destruct H0. congruence.
-destruct H0. destruct H0. destruct H0. destruct H0.
-destruct H1; congruence. 
+destruct H0. congruence.
+remember ((glob_types Delta) ! i). destruct o; simpl in *; try congruence. 
+unfold lift2 in *. right. unfold tc_ge_denote in H1.
+symmetry in Heqo2. 
+specialize (H1 _ _ Heqo2). destruct H1 as [b [i0 [? ?]]].
+rewrite <- H in *.  simpl ge_of in Heqo0. rewrite H1 in *.
+inv Heqo0. eauto. inv H2. 
 
-destruct H0. destruct H0. destruct H0. destruct H0.
-unfold proj_sumbool in *. destruct (type_eq t t1). subst.
-rewrite <- Heqo0 in H0. inv H0. eauto. inv H.
 
-inv H1. simpl in *. intuition. unfold lift1,lift2,lift0,force_ptr in *; destruct (eval_expr e rho); eauto.
+
+simpl in *. intuition. unfold lift1,lift2,lift0,force_ptr in *. 
+destruct (eval_expr e rho); eauto.
 
 simpl in *. unfold lift1,lift0,lift2 in *. intuition.
 unfold eval_field. unfold eval_struct_field.
@@ -653,28 +712,33 @@ simpl. subst; destruct t; auto; simpl in H0; inv H0; intuition.
 simpl in *. subst; destruct t; intuition. 
 
 (*Var*)
-st. unfold eval_var.  
+simpl in *. unfold eval_var.
 
-apply typecheck_environ_sound in H. destruct H.
-clear H. destruct H2. clear H2.
-unfold tc_ve_denote in *.
+assert (tc_mode_denote rho Delta ) as SM. unfold typecheck_environ in H. 
+rewrite andb_true_iff in H; intuition. apply typecheck_mode_eqv in H3. auto.
+destruct rho. 
+apply typecheck_environ_sound in H. destruct H as [_ [? ?]].
+unfold tc_ve_denote in *. unfold get_var_type in *. 
 
 remember ((var_types Delta) ! i).
-destruct o; try rewrite eqb_type_eq in *; simpl in *; intuition. (*if it isn't in delta, it won't typecheck*)
+destruct o; try rewrite eqb_type_eq in *; simpl in *; intuition. 
 unfold lift2 in H0.
-remember (type_eq t t0). destruct s; intuition. (*pt is type that the var lookup checks as*)
-subst. remember (negb(type_is_volatile t0)). destruct b; intuition.
+remember (type_eq t t0). destruct s; intuition. 
+subst. remember (negb(type_is_volatile t0)). destruct b; intuition. 
 clear H3. symmetry in Heqo.
 specialize (H i t0 Heqo).
 
-destruct H as [ [? ?] | [ [? [? [[? ?] [? ?]]]] | ? ]].  
+destruct H. 
 rewrite H in *. rewrite <- Heqb. rewrite eqb_type_refl in *. destruct pt; auto.
-remember (Map.get (ve_of rho) i). destruct o; try rewrite eqb_type_eq in *; simpl in *;  intuition.
-inv H3.  rewrite eqb_type_refl. rewrite <- Heqb. destruct pt; auto.
-rewrite H. rewrite eqb_type_refl. destruct pt; auto.
+remember ((glob_types Delta) ! i). destruct o; try congruence. 
+simpl in *. unfold lift2 in H0. destruct H0. remember (eqb_type t (globtype g)).
+symmetry in Heqb. destruct b; simpl in *; try congruence. apply eqb_type_true in Heqb.
+subst. unfold tc_mode_denote in *. symmetry in Heqo0.  specialize (SM _ _ Heqo0). 
+destruct SM. simpl in H4. unfold Map.get. rewrite H4. 
+unfold tc_ge_denote in *. edestruct H2; eauto. destruct H5. destruct H5. 
+rewrite H5. rewrite eqb_type_refl. auto. destruct H4; congruence.  
 
-destruct H as [? [? [[? ?] ?]]].
-rewrite H3. rewrite H. rewrite eqb_type_refl. destruct pt; auto.
+inv H0. inv H0. 
 
 (*Temp*)
 Focus 1.
@@ -686,12 +750,12 @@ unfold eval_id in *.
 simpl. unfold force_val.
 destruct Delta. destruct p. destruct p. 
 unfold temp_types in *. simpl in *.
-remember (t1 ! i). destruct o.
+remember (t2 ! i). destruct o.
   symmetry in Heqo.  
-  destruct p. specialize (H1 i t3 b Heqo). simpl in *.
+  destruct p. specialize (H1 i _ b Heqo). simpl in *.
   rewrite eqb_type_eq in *. destruct H1 as [? [? ?]].
   rewrite H. if_tac in H0; simpl in *; try solve [inv H0].
-  destruct (type_eq t t3); try solve [inv H0]. subst; auto.
+  destruct (type_eq t _); try solve [inv H0]. subst; auto.
   if_tac in H0; inv H0.
 
 (*deref*)  
@@ -777,16 +841,17 @@ try destruct i0; try destruct s; intuition; try destruct i1; try destruct s0; tr
 remember (typeof e1). unfold bool_val. destruct t0; intuition.*)
 
 (*EField*)
-st. unfold lift2,eval_field,eval_struct_field,lift1 in *; intuition. specialize  (H3 pt). intuition. remember rho.
+st. unfold lift2,eval_field,eval_struct_field,lift1 in *; intuition. 
+specialize  (H3 pt). intuition. remember rho.
 destruct e0.
-apply typecheck_environ_sound in H. intuition. clear H4 H8.
+apply typecheck_environ_sound in H. intuition. clear H4.
 rewrite Heqe0 in H0.
-assert (PTR := eval_lvalue_ptr _ _ _ _ _ _ Heqe0 H H0).
+assert (PTR := eval_lvalue_ptr _ e _ _ _ _ Heqe0 H H8).
 rewrite Heqe0 in *. clear Heqe0.
 intuition. 
 remember (eval_lvalue e rho). unfold denote_tc_isptr in *.
 destruct v; intuition; try congruence.
-remember (eval_lvalue e rho). destruct H4. destruct H4.
+remember (eval_lvalue e rho). destruct H7. destruct H4.
 destruct v; intuition; try congruence.
 inv H4.
 destruct (typeof e); intuition. 
@@ -1017,9 +1082,11 @@ try solve[intuition; constructor; auto | subst; inv H1]; intuition.
 (* var*)
 assert (TC_Sound:= typecheck_lvalue_sound).
 specialize (TC_Sound Delta rho (Evar i t) H0 H1).
-specialize (TC_Sound some_pt_type).
+specialize (TC_Sound some_pt_type). simpl in TC_Sound.
+specialize (TC_Sound (eq_refl _)). 
  
-st. unfold eval_var in *. remember (Map.get (ve_of rho) i); destruct o; try destruct p; 
+simpl in *. unfold eval_var in *. 
+remember (Map.get (ve_of rho) i); destruct o; try destruct p; 
 try rewrite eqb_type_eq in *; simpl in *.
 destruct (type_eq t t0); simpl in *; intuition.
 subst t0. if_tac; intuition.
@@ -1031,34 +1098,42 @@ remember (ge_of rho i). destruct o; try destruct p; auto;
 try rewrite eqb_type_eq in *; simpl in *; intuition.
 destruct (type_eq t t0); simpl in *. subst t0.
 
+unfold get_var_type in *. 
 remember ((var_types Delta) ! i). 
 destruct o; try rewrite eqb_type_eq in *; simpl in *; unfold lift2 in *; intuition.
 destruct (type_eq t t0); simpl in *; [ | contradiction]. subst t0.
-symmetry in Heqo1. 
+symmetry in Heqo1.
+destruct rho.  
 apply typecheck_environ_sound in H0.
 intuition. unfold tc_ve_denote in *. 
-specialize (H0 i t Heqo1). 
-rewrite <- Heqo in *. rewrite <- Heqo0 in *. intuition. destruct H5. congruence.
-repeat destruct H0. destruct H5. congruence.
- destruct v; intuition. destruct H0. destruct H0.
-intuition. congruence. destruct H0. destruct H0. intuition.
-inv H0. exists x. exists x0. intuition. simpl in *.
-symmetry in Heqo0.
-assert (Eq := filter_genv_zero_ofs _ _ x x0 t (eq_refl _) _ Heqo0). subst.
-apply Clight_sem.eval_Evar_global; auto. 
-unfold filter_genv in Heqo0. 
-destruct (Genv.find_symbol ge i). destruct ( type_of_global ge b).
-inv Heqo0. auto. inv Heqo0. auto. congruence.
-unfold filter_genv in Heqo0. destruct (Genv.find_symbol ge i); try congruence.
-assert (x = b). destruct (type_of_global ge b); inv Heqo0; auto.
-subst. 
-destruct (type_of_global ge b). inv Heqo0. auto. inv Heqo0. congruence.
-congruence.
+unfold tc_ge_denote in *. 
+specialize (H0 i t Heqo1). unfold ge_of in *. unfold Map.get in *. 
+destruct H0. simpl in Heqo. congruence.
 
-(*temp*)
+destruct rho. 
+apply typecheck_environ_sound in H0. intuition. unfold tc_ge_denote in *. 
+remember ((glob_types Delta) ! i). destruct o; simpl in H1; try congruence.
+unfold lift2 in *. destruct H1. 
+symmetry in Heqo2. specialize (H4 _ _ Heqo2).  destruct H4. destruct H4. 
+destruct H4. simpl in Heqo0. rewrite H4 in *. inv Heqo0. exists x. exists x0. split; auto. 
+unfold construct_rho in *. inv H. simpl in Heqo. clear H1. 
+remember (filter_genv ge). symmetry in Heqg0. 
+assert (ZO := filter_genv_zero_ofs _ _ _ _ _ Heqg0 _ H4).  subst.
+apply Clight_sem.eval_Evar_global. auto.  unfold filter_genv in H4.
+destruct (Genv.find_symbol ge i). destruct (type_of_global ge b); inv H4; auto. 
+congruence.  
+
+unfold filter_genv in H4.
+remember (Genv.find_symbol ge i).  destruct o; try congruence.  
+assert (x = b). destruct (type_of_global ge b); inv H4; auto. subst.
+destruct (type_of_global ge b). inv H4; auto. inv H4. rewrite <- H1 in *. simpl in *.
+congruence. 
+intuition. congruence. 
+
+(*temp*)  
 assert (TC:= typecheck_expr_sound).
 specialize (TC Delta rho (Etempvar i t)). simpl in *. 
-intuition.
+intuition.  
 constructor. unfold eval_id in *. remember (Map.get (te_of rho)  i);
 destruct o;  auto. destruct rho; inv H; unfold make_tenv in *.
 unfold Map.get in *. auto. 
@@ -1079,10 +1154,11 @@ simpl in H1. unfold lift2 in *.
 assert (ISPTR := eval_lvalue_ptr rho e Delta (te_of rho) (ve_of rho) (ge_of rho)).
 specialize (IHe ge).
 assert (mkEnviron (ge_of rho) (ve_of rho) (te_of rho) = rho). destruct rho; auto.
+destruct rho. 
 intuition; apply typecheck_environ_sound in H0. intuition. 
-simpl. destruct H7. destruct H1. intuition. congruence. 
-destruct H7. destruct H1. destruct H1. destruct H8. destruct H8.  simpl in *.
-intuition. rewrite H8. constructor. rewrite H8 in H7. inversion H7. auto.
+simpl. destruct H7. destruct H7. intuition. congruence. 
+destruct H7. destruct H7. destruct H7. destruct H1. destruct H1.  simpl in *.
+intuition. rewrite H8 in *. constructor. inv H1. auto.
 
 (*unop*)
 simpl in *. unfold lift1,lift2,eval_unop in *. intuition. unfold force_val. 
@@ -1193,16 +1269,21 @@ type_is_volatile (typeof e) = false.
 Proof.
 intros.
 destruct e; intuition; simpl in *. 
+unfold get_var_type in *. 
 
 destruct ((var_types Delta) ! i); intuition; simpl in *. unfold lift2 in *;
 intuition. unfold tc_bool in *. rewrite if_negb in *.
 if_tac in H1; simpl in *; unfold lift2 in *; intuition.
 
 unfold lift2 in *; intuition. unfold tc_bool in *. rewrite if_negb in *.
-if_tac in H1; intuition.
+destruct ((glob_types Delta) ! i). simpl in *. unfold lift2 in *. 
+destruct H. if_tac in H0; auto; inv H0. inv H. 
 
 unfold lift2 in *; intuition. clear - H1. unfold tc_bool in *. rewrite if_negb in *.
 if_tac in H1; intuition.
+
+unfold lift2 in *. intuition. unfold tc_bool in *.  rewrite if_negb in *. 
+if_tac in H1; auto. inv H1. 
 Qed.
 
 (*Proof for "backwards environment checking" that an environment that typechecks
@@ -1240,6 +1321,7 @@ apply IHl; auto; intros. rewrite H in *. inv H3. specialize (H2 (t1, b1)).
 intuition. inv H2. congruence.
 Qed.
 
+(* Should be unneeded, we never change ve on join
 Lemma join_ve_eqv :forall ve1 ve2 id v,
 ve1 ! id = Some v -> ve2 ! id = Some v ->
 (join_ve ve1 ve2) ! id = Some v.
@@ -1265,16 +1347,7 @@ apply IHl; auto; intros. rewrite H in *. inv H3. specialize (H2 t0).
 intuition. inv H2. congruence.
 
 Qed.
-
-Lemma join_vl_eqv : forall vl1 vl2 id,
-In id vl1 -> In id vl2 -> In id (join_ve_list vl1 vl2).
-Proof.
-intros.
-induction vl1. inv H.
-destruct H. subst. unfold join_ve_list. simpl.
-if_tac. simpl. auto. intuition. 
-simpl. if_tac; intuition.
-Qed.
+*)
 
 Lemma temp_types_same_type : forall id i t b Delta,
 (temp_types Delta) ! id = Some (t, b) ->
@@ -1300,16 +1373,7 @@ Qed.
 
 Lemma var_types_update_dist : forall d1 d2 ,
 (var_types (join_tycon (d1) (d2))) =
-join_ve (var_types (d1)) (var_types (d2)).
-Proof.
-intros.
-destruct d1; destruct d2. destruct p; destruct p0. destruct p0; destruct p.
-simpl. unfold var_types. simpl. auto.
-Qed.
-
-Lemma non_var_ids_update_dist : forall d1 d2 ,
-(non_var_ids (join_tycon (d1) (d2))) =
-join_ve_list (non_var_ids (d1)) (non_var_ids (d2)).
+(var_types (d1)).
 Proof.
 intros.
 destruct d1; destruct d2. destruct p; destruct p0. destruct p0; destruct p.
@@ -1395,7 +1459,7 @@ destruct (update_tycon_te_same c1 _ _ _ _ H0).
 destruct (update_tycon_te_same c2 _ _ _ _ H0).
  eapply H. unfold join_tycon. remember (update_tycon Delta c1).
 destruct t. destruct p. destruct p. remember (update_tycon Delta c2).
-destruct t2. destruct p. destruct p. unfold temp_types in *.
+destruct t3. destruct p. destruct p. unfold temp_types in *.
 unfold update_tycon. simpl in *.
 
 apply join_te_eqv; eauto.    
@@ -1419,19 +1483,20 @@ Lemma set_temp_ve : forall Delta i,
 var_types (initialized i Delta) = var_types (Delta).
 Proof.
 intros. destruct Delta. destruct p. destruct p. unfold var_types. unfold initialized.
-simpl. unfold temp_types. simpl. destruct (t0 ! i); auto. destruct p; auto.
+simpl. unfold temp_types. simpl. destruct (t1 ! i); auto. destruct p; auto.
 Qed. 
 
-Lemma set_temp_vl : forall Delta i,
-non_var_ids (initialized i Delta) = non_var_ids (Delta).
+Lemma set_temp_ge : forall Delta i,
+glob_types (initialized i Delta) = glob_types (Delta).
 Proof.
 intros. destruct Delta. destruct p. destruct p. unfold var_types. unfold initialized.
-simpl. unfold temp_types. simpl. destruct (t0 ! i); auto. destruct p; auto.
+simpl. unfold temp_types. simpl. destruct (t1 ! i); auto. destruct p; auto.
 Qed. 
 
 Lemma update_tycon_same_ve : forall Delta c id v,
 (var_types (update_tycon Delta c)) ! id = Some v <->
 (var_types (Delta)) ! id = Some v
+
 
 with update_le_same_ve : forall (l : labeled_statements) (id : positive) (v : type) Delta,
 (var_types (join_tycon_labeled l Delta)) ! id = Some v <->
@@ -1443,30 +1508,79 @@ rewrite set_temp_ve in H. auto.
 destruct o. rewrite set_temp_ve in H. auto.
 auto.
 eapply update_tycon_same_ve. rewrite <- update_tycon_same_ve. apply H.
-rewrite var_types_update_dist in H. apply join_ve_denote in H.
-destruct H. rewrite update_tycon_same_ve in H. auto.
+
+rewrite var_types_update_dist in H.
+rewrite update_tycon_same_ve in H. auto.
 rewrite update_tycon_same_ve in H. apply H.
 erewrite update_le_same_ve in H. apply H.
 
 destruct c; simpl in *; try apply H. rewrite set_temp_ve. apply H.
 destruct o. rewrite set_temp_ve. apply H.
 apply H. rewrite update_tycon_same_ve. rewrite update_tycon_same_ve.
-apply H. rewrite var_types_update_dist. apply join_ve_eqv.
+apply H. rewrite var_types_update_dist. 
 rewrite update_tycon_same_ve. apply H. rewrite update_tycon_same_ve.
-apply H. rewrite update_tycon_same_ve. apply H.
+apply H. 
 rewrite update_le_same_ve. apply H.
 
 intros. split. intros.
  destruct l. simpl in *. rewrite update_tycon_same_ve in H.
 apply H. simpl in *. rewrite var_types_update_dist in H.
-apply join_ve_denote in H. destruct H. rewrite update_tycon_same_ve in H. apply H.
+rewrite update_tycon_same_ve in H. apply H.
 
 intros. destruct l; simpl in *.
 rewrite update_tycon_same_ve. apply H.
-rewrite var_types_update_dist. apply join_ve_eqv. rewrite update_tycon_same_ve.
-apply H. apply update_le_same_ve. apply H.
+rewrite var_types_update_dist.  rewrite update_tycon_same_ve.
+apply H.
 Qed.   
 
+
+Lemma glob_types_update_dist :
+ forall d1 d2 : tycontext, glob_types (join_tycon d1 d2) = glob_types d1.
+destruct d1; destruct d2.  destruct p. destruct p. destruct p0. destruct p. 
+auto. 
+Qed.
+
+Lemma update_tycon_same_ge : forall Delta c id v,
+(glob_types (update_tycon Delta c)) ! id = Some v <->
+(glob_types (Delta)) ! id = Some v
+
+
+with update_le_same_ge : forall (l : labeled_statements) (id : positive) (v : global_spec) Delta,
+(glob_types (join_tycon_labeled l Delta)) ! id = Some v <->
+(glob_types Delta) ! id = Some v.
+Proof.
+intros; split; intros.
+destruct c; simpl in *; try apply H.
+rewrite set_temp_ge in H. auto.
+destruct o. rewrite set_temp_ge in H. auto.
+auto.
+eapply update_tycon_same_ge. rewrite <- update_tycon_same_ge. apply H.
+
+rewrite glob_types_update_dist in H.
+rewrite update_tycon_same_ge in H. auto.
+rewrite update_tycon_same_ge in H. apply H.
+erewrite update_le_same_ge in H. apply H.
+
+destruct c; simpl in *; try apply H. rewrite set_temp_ge. apply H.
+destruct o. rewrite set_temp_ge. apply H.
+apply H. rewrite update_tycon_same_ge. rewrite update_tycon_same_ge.
+apply H. rewrite glob_types_update_dist. 
+rewrite update_tycon_same_ge. apply H. rewrite update_tycon_same_ge.
+apply H. 
+rewrite update_le_same_ge. apply H.
+
+intros. split. intros.
+ destruct l. simpl in *. rewrite update_tycon_same_ge in H.
+apply H. simpl in *. rewrite glob_types_update_dist in H.
+rewrite update_tycon_same_ge in H. apply H.
+
+intros. destruct l; simpl in *.
+rewrite update_tycon_same_ge. apply H.
+rewrite glob_types_update_dist.  rewrite update_tycon_same_ge.
+apply H.
+Qed.   
+
+(*should be unneeded now
 Lemma ve_join_update :
 (forall (rho : environ) (c : statement) (Delta : tycontext),
  tc_ve_denote (ve_of rho) (ge_of rho) (var_types (update_tycon Delta c)) ->
@@ -1491,16 +1605,15 @@ rewrite update_tycon_same_ve. apply H1.
 assert (t4 = var_types (update_tycon Delta c2)).
 rewrite <- Heqt2; unfold var_types; auto. subst.
 rewrite update_tycon_same_ve. apply H1.
-Qed.
+Qed.*)
 
 
 Lemma typecheck_environ_update_ve : forall (rho : environ) (c : statement) (Delta : tycontext),
-tc_ve_denote (ve_of rho) (ge_of rho) (var_types (update_tycon Delta c)) ->
-tc_ve_denote (ve_of rho) (ge_of rho) (var_types Delta).
+tc_ve_denote (ve_of rho) (var_types (update_tycon Delta c)) ->
+tc_ve_denote (ve_of rho) (var_types Delta).
 Proof.
 intros. destruct c; simpl in *; try apply H;
 try destruct o; try rewrite set_temp_ve in *; try apply H;
-
 unfold tc_ve_denote in *; intros; apply H; try rewrite var_types_update_dist; 
 try apply join_ve_eqv;
 repeat rewrite update_tycon_same_ve in *; try rewrite update_le_same_ve;
@@ -1508,53 +1621,39 @@ auto.
 Qed. 
 
 
-Lemma typecheck_environ_update_vl : 
-forall (c : statement) (Delta : tycontext) (id : positive),
-In id (non_var_ids Delta) -> In id (non_var_ids (update_tycon Delta c))
 
-with typecheck_le_update_vl :
-forall (l : labeled_statements) (Delta : tycontext) (id : positive),
-In id (non_var_ids Delta) -> In id (non_var_ids (join_tycon_labeled l Delta)).
-Proof. 
-destruct c; intros; simpl in *; try destruct o; try rewrite set_temp_vl; try apply H.
-
-apply typecheck_environ_update_vl. apply typecheck_environ_update_vl.
-apply H.
-
-rewrite non_var_ids_update_dist. apply join_vl_eqv. apply typecheck_environ_update_vl.
-apply H.
-
-apply typecheck_environ_update_vl. apply H.
-
-apply typecheck_environ_update_vl. apply H.
-
-apply typecheck_le_update_vl. apply H.
-
-intros. destruct l; simpl in *. apply typecheck_environ_update_vl; apply H.
-rewrite non_var_ids_update_dist. apply join_vl_eqv. apply typecheck_environ_update_vl.
-apply H.
-apply typecheck_le_update_vl. apply H.
-Qed.
-
+Lemma typecheck_environ_update_ge : forall (rho : environ) (c : statement) (Delta : tycontext),
+tc_ge_denote (ge_of rho) (glob_types (update_tycon Delta c)) ->
+tc_ge_denote (ge_of rho) (glob_types Delta).
+Proof.
+intros. destruct c; simpl in *; try apply H;
+try destruct o; try rewrite set_temp_ge in *; try apply H;
+unfold tc_ge_denote in *; intros; apply H; try rewrite glob_types_update_dist; 
+try apply join_ge_eqv;
+repeat rewrite update_tycon_same_ge in *; try rewrite update_le_same_ge;
+auto.
+Qed. 
 
 Lemma typecheck_environ_update:
   forall rho c Delta, typecheck_environ rho (update_tycon Delta c) = true ->
        typecheck_environ rho Delta = true.
 Proof.
-intros. unfold typecheck_environ in *. repeat rewrite andb_true_iff in *.
-destruct H. destruct H. split. split. clear H0 H1.
-rewrite typecheck_te_eqv in *. eapply typecheck_environ_update_te; eauto.
+intros. unfold typecheck_environ in *. repeat rewrite andb_true_iff in *. 
+destruct H. destruct H. destruct H.  split. split. split. clear H0 H1 H2.
+rewrite typecheck_te_eqv in *.  intuition.  eapply typecheck_environ_update_te; eauto.
 
-rewrite typecheck_ve_eqv in *. clear H H0. eapply typecheck_environ_update_ve.
+clear H H0 H1. 
+rewrite typecheck_ve_eqv in *. eapply typecheck_environ_update_ve.
 eauto.
 
+clear H H0 H2. rewrite typecheck_ge_eqv in *. eapply typecheck_environ_update_ge.
+eauto.  
 
-rewrite typecheck_vl_eqv in *. clear H H1. unfold tc_vl_denote in *.
-intros. apply H0. clear H0. apply typecheck_environ_update_vl.
-apply H.
+clear -H0.  assert (TM := typecheck_mode_eqv rho Delta). apply TM.  
+admit.  (* rewrite typecheck_mode_eqv. *)
+
 Qed.
 
-(* Admitted: move this to expr.v or something *)
 Lemma typecheck_bool_val:
   forall v t, typecheck_val v t = true -> bool_type t = true ->
       exists b, strict_bool_val v t = Some b.
